src/sys_verif/program_proof/ghost_state.v
@@ -1,0 +1,259 @@
+(*| # Lecture 19: Ghost state
+
+> Follow these notes in Coq at [src/sys_verif/program_proof/ghost_state.v](https://github.com/tchajed/sys-verif-fa24-proofs/blob/main/src/sys_verif/program_proof/ghost_state.v).
+
+## Learning outcomes
+
+1. Explain the API for a ghost variable.
+2. Use ghost state for simple concurrency proofs.
+
+<!-- @include: ./macros.snippet.md -->
+
+## Motivation
+
+Resource algebras gave a way to share locations among threads, at least read-only. This turns out not to be enough to prove reasonable programs; we'll have a running example of something apparently simple that requires new techniques.
+
+Not to fear, though, since _more_ resource algebras will solve the problem. Instead of just using RAs to divide ownership of (physical) pointers, we can also use them to divide ownership of _ghost variables_ that are only created for the sake of the proof.
+
+## Code example
+
+```go
+// JoinHandle is a mechanism to wait for a goroutine to finish. Calling `Join()`
+// on the handle returned by `Spawn(f)` will wait for f to finish.
+type JoinHandle struct {
+  /* private fields */
+}
+
+// Spawn runs `f` in a parallel goroutine and returns a handle to wait for
+// it to finish.
+func Spawn(f func()) *JoinHandle
+
+// ParallelAdd3 adds 2 to a shared integer from two threads, then reads the
+// result.
+//
+// It returns 4.
+//
+// The 3 in the name is because there are two earlier versions of this example
+// with slightly different concurrency primitives.
+func ParallelAdd3() uint64 {
+	m := new(sync.Mutex)
+	var i uint64 = 0
+	h1 := std.Spawn(func() {
+		m.Lock()
+		i = std.SumAssumeNoOverflow(i, 2)
+		m.Unlock()
+	})
+	h2 := std.Spawn(func() {
+		m.Lock()
+		i = std.SumAssumeNoOverflow(i, 2)
+		m.Unlock()
+	})
+	h1.Join()
+	h2.Join()
+	m.Lock()
+	y := i
+	m.Unlock()
+	return y
+}
+```
+
+What could the lock invariant be?
+
+### Exercise: come up with a lock invariant
+
+Try to come up with a lock invariant to prove that the result is exactly 4. Then, after failing to do that, come up with a lock invariant that is at least true.
+
+## Ghost variables
+
+### Syntax
+
+Ghost variables build upon the general support for RAs we used to develop fractional permissions.
+
+We need one tweak to separation logic assertions to support talking about ghost variables: instead of a single global RA $\own(a)$, which we only used to define $l \mapsto_q v$, we'll define $\own_\gamma(a : M)$ for ownership of $a$ within a ghost variable named $\gamma$ (gamma) that has type $M$, which is an RA.
+
+Note that:
+
+1. We can have several ghost variables, as indicated by the presence of a name (we'll see that these variables can be dynamically allocated).
+2. The value of a ghost variable is an element of a resource algebra.
+3. We can pick an arbitrary RA for each ghost variable, and a different one for each.
+
+It's worth commenting right away on the difference between $\own_γ(a : M)$ and the value of the ghost variable. It's helpful to think of a ghost variable as having some global value, but ownership of that value can be subdivided according to $\own_γ(a \cdot b) ⊣⊢ \own_γ(a) ∗ \own_γ(b)$ (with the definition of $\cdot$ coming from $M$), and then those separate $\own_γ$ assertions could be divided among threads or put into lock invariants. The value of the ghost variable $γ$ is the composition of all the parts of all the threads at any given point in time.
+
+### Creating and modifying ghost variables
+
+An important aspect of ghost variables is when they can be changed. This is non-trivial because we can split ownership of a ghost variable, so it's important that changes in one "shard" (that is, one $\own_\gamma$) are consistent with the other shards.
+
+To see the importance of this consistency, consider ghost variables using the fracRA from last lecture. Recall that the elements had the form $(q, v)$, and composition was defined as follows: $(q_1, v) \cdot (q_2, v) = (q_1 + q_2, v)$ and $(q_1, v_1) \cdot (q_2, v_2) = \errorval$ if $v_1 ≠ v_2$. If we split $\own_γ((1, v))$ into $\own_γ((1/2, v)) ∗ \own_γ((1/2, v))$ and change just one half to $\own_γ((1/2, v'))$, what happens?
+
+**Exercise:** Think for a minute about what goes wrong.
+
+::: details Solution
+
+If at one step of the proof we had $\own_γ((1, v)) ⊢ \own_γ((1/2, v)) ∗ \own_γ((1/2), v)$ and then somehow changed one half, the other is presumably unaffected (since it is separate). Then we'd have $\own_\gamma((1/2, v')) ∗ \own_γ((1/2, v))$. These can be recombined to form $\own_γ(\errorval)$. But we know that all owned values are valid, so we have now proven $\lift{\False}$. If a program proof could take this action, it could prove anything, and we know that this would make separation logic unsound.
+
+:::
+
+The rule for changing ghost variables is that the allowed changes are _frame-preserving updates_. A frame-preserving update $a \mupd b$ is one where $∀ r, \valid (a \cdot r) → \valid (b \cdot r)$. First, let's informally understand why this would make sense. Remember that in our proofs we're going to maintain that the ghost variable's value is always _valid_ according to $✓(a)$ from the RA. Also recall that while one thread might have $\own_γ(a)$, the ghost variable can have other parts in other threads (as we just saw in the problematic example). What a frame-preserving update says is, if a thread has $a$ and other threads own $r$, for any such $r$ where the composition is valid (and thus that is actually possible), then changing $a$ to $b$ retains validity of the whole ghost variable. This is what guarantees that changes don't invalidate any ownership in other threads, or the global ghost variable.
+
+To use a frame-preserving update, we need to introduce the _update modality_ $\pvs P$ (pronounced "update P"). You've already seen this come up in Coq proofs as `|==>` and ignored it with `iModIntro`.
+
+Whenever $a \mupd b$ (there is a frame preserving update from $a$ to $b$), what we formally get in the logic is an entailment $\own_γ(a) ⊢ \pvs \own_γ(b)$. The intuitive reading of the whole entailment is easier to start with than the update modality in isolation: it's possible to change ghost state so that if $\own_γ(a)$ was true before, afterward $\own_γ(b)$ is true. It's not the case that $\own_γ(a) ⊢ \own_γ(b)$; you should think of the update as actually changing (ghost) state, and $b$ isn't true previously. However, for practical purposes we'll see that while verifying a program $\pvs P$ can be turned into $P$.
+
+The next API we need for ghost variables is to allocate them initially. The rule for this is fairly simple: $∀ a, \lift{✓(a)} ⊢ \pvs ∃ γ, \own_γ(a)$. This says that we can always change ghost state (that's the reading of the $\pvs$) to create a new variable with some name $γ$, and its initial value is any valid element $a$.
+
+Let's start seeing some examples of ghost variables and their updates in Coq.
+
+|*)
+
+From sys_verif.program_proof Require Import prelude empty_ffi.
+From Perennial.algebra Require Import ghost_var.
+From Perennial.program_proof Require Import std_proof.
+From Goose.sys_verif_code Require Import concurrent.
+
+Section goose.
+Context `{hG: !heapGS Σ}.
+Context `{ghost_varG0: ghost_varG Σ Z}.
+Open Scope Z_scope.
+
+(*| The first example we'll see is so-called "plain" ghost variables, which have a value and a fraction, and the fraction can be split. This is just like our fracRA example.
+
+The library hides the literal `own` construct in Iris behind some sealing machinery. Despite this, we can still print its definition with the following:
+|*)
+Print ghost_var.ghost_var_def.
+
+(*| The actual value passed to `own` uses `dfrac_agree.to_frac_agree`, which constructs an element of the dfrac_agree RA; that's the actual RA as defined in Iris.
+
+---
+
+|*)
+
+Lemma ghost_var_change_ex1 γ :
+  ghost_var γ (DfracOwn 1) 7%Z -∗ |==> ghost_var γ (DfracOwn 1) 23%Z.
+Proof.
+  iIntros "H".
+  (* We use `iMod` to "execute" a ghost update. This is only legal because the
+  goal allows it, which is true for a goal that starts with `|==>` (as we have
+  here) or a WP goal. *)
+  iMod (ghost_var_update 23%Z with "H") as "H".
+  (* _After_ we're done doing ghost updates, we can remove the update modality
+  from the goal with iModIntro. *)
+  iModIntro.
+  iExact "H".
+Qed.
+
+(*| Here's a special case allocation lemma for this particular type of ghost state. (I'm using `@ghost_var_alloc Σ` rather than `ghost_var_alloc` to reduce some noise in the output.) |*)
+Check (@ghost_var_alloc Σ).
+
+(*| For our second example of an RA and its ghost variables, let's look at _discardable fractions_ (dfrac). You've seen `DfracOwn 1` instead of just the fraction 1; now we'll see (roughly) how that works.
+
+Discardable fractions are like fractions between 0 and 1 (excluding 0, including 1), with the addition of a special $ε$ value, called `DfracDiscarded`. You can see a more complete description in the RA lecture's [discardable fractions section](./resource-algebra#discardable-fractions), or look at the definition of dfrac in Iris for actually all of the details.
+
+Discardable fractions are used in the ghost variable API: instead of composing fractions with $q_1 + q_2$, we're actually using $dq_1 : \mathrm{dfrac}$ and composing with dfrac composition $dq_1 \cdot dq_2$ (which does still behave a lot like addition).
+
+For this discussion there are two salient aspects of dfrac composition:
+
+- $∀ dq, ✓(dq) → dq \mupd ε$. This means that it is valid to change any fraction to the value $ε$.
+- $∀ (dq: \mathrm{dfrac}), ε \cdot ε = ε$. This makes owning a discarded $ε$ duplicable (and actually it is _persistent_).
+
+The first is the "discard" part of discardable fractions, and it means we have the following ghost update:
+
+|*)
+
+Check (@ghost_var_persist Σ).
+
+(*| The second is what makes discardable fractions especially useful: |*)
+
+Check (@ghost_var_persistent Σ).
+
+(*| ### Proof of the example
+
+Let's put this together to verify the parallel add example. We'll use an existing spec for the Spawn/JoinHandle API, lock invariants, and two ghost variables.
+
+|*)
+
+(*| The essence of the proof is really in the lock invariant. `l` here is the address of the `x` variable in the Go code.
+
+The idea is that the two variables correspond to the component each thread has added to the shared variable. the lock owns half of each variable; the first thread has the other half of `γ1` and the second thread has the other half of `γ2`.
+
+The lock invariant also connects all of this ghost state back to the physical state: the value stored in `l` is the sum of the two ghost variables.
+
+We also maintain that both ghost variables are less than 2 so that we can prove the additions don't overflow.
+
+|*)
+Definition lock_inv γ1 γ2 l : iProp _ :=
+  ∃ (x: w64) (x1 x2: Z),
+    "Hx1" :: ghost_var γ1 (DfracOwn (1/2)) x1 ∗
+    "Hx2" :: ghost_var γ2 (DfracOwn (1/2)) x2 ∗
+    "x" ∷ l ↦[uint64T] #x ∗
+    "%Hsum" ∷ ⌜x1 ≤ 2 ∧ x2 ≤ 2 ∧ uint.Z x = (x1 + x2)%Z⌝.
+
+Lemma wp_ParallelAdd3 :
+  {{{ True }}}
+    ParallelAdd3 #()
+  {{{ (x: w64), RET #x; ⌜uint.Z x = 4⌝ }}}.
+Proof using All.
+  wp_start as "_".
+  iMod (ghost_var_alloc 0) as (γ1) "[Hv1_1 Hx1_2]".
+  iMod (ghost_var_alloc 0) as (γ2) "[Hv2_1 Hx2_2]".
+
+  (*| This proof illustrates one more thing, incidentally. The code creates a mutex before the variable `x` that it protects. This turns out not to be an issue; the Goose mutex specifications support this use case. What we do is first create a "free lock", which is a lock without a lock invariant (yet). |*)
+
+  wp_apply wp_new_free_lock; iIntros (mu_l) "Hlock".
+  wp_alloc x_l as "x".
+  iMod (alloc_lock nroot _ _ (lock_inv γ1 γ2 x_l)
+         with "Hlock [$x $Hv1_1 $Hv2_1]") as "#Hlock".
+  { iPureIntro. done. }
+  wp_pures.
+  (*| Observe here that the `alloc_lock` above has consumed the `is_free_lock` and associated it with a chosen lock invariant. Importantly, we couldn't actually use the `wp_Mutex__Lock` specification before using `alloc_lock`. |*)
+  wp_apply (std_proof.wp_Spawn (ghost_var γ1 (DfracOwn (1/2)) 2) with "[Hx1_2]").
+  {
+    clear Φ.
+    iIntros (Φ) "HΦ".
+    wp_pures.
+    wp_apply (wp_Mutex__Lock with "[$Hlock]"). iIntros "[locked Hinv]". iNamed "Hinv".
+    wp_load.
+    wp_store.
+    iDestruct (ghost_var_agree with "Hx1_2 Hx1") as %Heq; subst.
+    iMod (ghost_var_update_2 2 with "Hx1_2 Hx1") as "[Hx1_2 Hx1]".
+    { rewrite dfrac_op_own Qp.half_half //. }
+    wp_apply (wp_Mutex__Unlock with "[-HΦ Hx1_2 $Hlock $locked]").
+    { iFrame.
+      iPureIntro. split_and!; try word. }
+    wp_pures.
+    iApply "HΦ". iFrame. done.
+  }
+  iIntros (h_1) "h1".
+  wp_apply (std_proof.wp_Spawn (ghost_var γ2 (DfracOwn (1/2)) 2) with "[Hx2_2]").
+  {
+    clear Φ.
+    iIntros (Φ) "HΦ".
+    wp_pures.
+    wp_apply (wp_Mutex__Lock with "[$Hlock]"). iIntros "[locked Hinv]". iNamed "Hinv".
+    wp_load.
+    wp_store.
+    iDestruct (ghost_var_agree with "Hx2_2 Hx2") as %Heq; subst.
+    iMod (ghost_var_update_2 2 with "Hx2_2 Hx2") as "[Hx2_2 Hx2]".
+    { rewrite dfrac_op_own Qp.half_half //. }
+    wp_apply (wp_Mutex__Unlock with "[-HΦ Hx2_2 $Hlock $locked]").
+    { iFrame.
+      iPureIntro. split_and!; try word. }
+    wp_pures.
+    iApply "HΦ". iFrame. done.
+  }
+  iIntros (h_2) "h2".
+  wp_pures.
+  wp_apply (wp_JoinHandle__Join with "[$h1]"). iIntros "Hx1_2".
+  wp_apply (wp_JoinHandle__Join with "[$h2]"). iIntros "Hx2_2".
+  wp_apply (wp_Mutex__Lock with "[$Hlock]"). iIntros "[locked Hinv]". iNamed "Hinv".
+  iDestruct (ghost_var_agree with "Hx1_2 Hx1") as %Heq; subst.
+  iDestruct (ghost_var_agree with "Hx2_2 Hx2") as %Heq; subst.
+  wp_load.
+  wp_apply (wp_Mutex__Unlock with "[$locked $Hlock Hx1 Hx2 x]").
+  { iFrame. iPureIntro. split_and!; word. }
+  wp_pures.
+  iModIntro.
+  iApply "HΦ".
+  iPureIntro. word.
+Qed.
+
+End goose.
